proofs/NoAImpliesNoFly/NoAImpliesNoFlyLinked.v
@@ -2836,6 +2836,7 @@ Section NoARealInputMWF.
                             Hpres_warp_ext))
                       Hcp_pas
                       (Hpres_obj_ext mario._set_camera_mode eq_refl)
+                      (Hpres_obj_ext interaction._set_camera_shake_from_hit eq_refl)
                       Hpres_cut_rest))
                 (automatic_pres lp LO_mario LO_aut bm (NoA_real bm)
                    (MWF_real lp bm bc oc0 SafeB)
